@prefix dct:       <http://purl.org/dc/terms/> .
@prefix foaf:      <http://xmlns.com/foaf/0.1/> .
@prefix owl:       <http://www.w3.org/2002/07/owl#> .
@prefix prov:      <http://www.w3.org/ns/prov#> .
@prefix rdf:       <http://www.w3.org/1999/02/22-rdf-syntax-ns#> .
@prefix rdfs:      <http://www.w3.org/2000/01/rdf-schema#> .
@prefix xsd:       <http://www.w3.org/2001/XMLSchema#>.

@prefix fua:       <https://www.nicos-rd.com/fua#> .
@prefix form:      <https://www.nicos-rd.com/fua/form#> .

form:
    a                owl:Ontology ;
    rdfs:label       "Form Ontology"@en ;
    dct:description  """
        This ontology defines a set of classes and properties to describe a form.
        It can be used for any survey, questionnaire or interview.
        The ontology does not only contain a model for questions but for answers as well.
    """@en ;
    rdfs:isDefinedBy form: ;
.

form:Questionnaire
    a                owl:Class ;
    rdfs:label       "Questionnaire"@en ;
    dct:description  """
        The questionnaire is the root object that contains all questions and sections.
        Although the questionnaire can contain questions, it is advised to use sections for structuring.
        If a questionnaire is answered, a corresponding questionnaire result must be created.
    """@en ;
    rdfs:isDefinedBy form: ;
.

form:Section
    a                owl:Class ;
    rdfs:label       "Section"@en ;
    dct:description  """
        The section groups multiple questions in a questionnaire together.
        It is only meant to group questions together for easier visibility.
        A section can contain sub-sections, but it can also contain questions directly.
    """@en ;
    rdfs:isDefinedBy form: ;
.

form:section
    a                owl:ObjectProperty ;
    rdfs:label       "section"@en ;
    dct:description  """
        The section property is used with the questionnaire and section class to structure the questions.
    """@en ;
    rdfs:domain      [ a           owl:Class ;
                       owl:unionOf ( form:Questionnaire
                                     form:Section ) ; ] ;
    rdfs:range       form:Section ;
    rdfs:isDefinedBy form: ;
.

form:Question
    a                owl:Class ;
    rdfs:label       "Question"@en ;
    dct:description  """
        The question is the smalled individual in a questionnaire and defines what should be asked in the form.
        Different sub-classes are used to differentiate different types of form questions.
    """@en ;
    rdfs:isDefinedBy form: ;
.

form:question
    a                owl:ObjectProperty ;
    rdfs:label       "question"@en ;
    dct:description  """
        The question property is used with the questionnaire and section class to structure the questions.
        The property is also used to reference a question from an answer.
    """@en ;
    rdfs:domain      [ a           owl:Class ;
                       owl:unionOf ( form:Questionnaire
                                     form:Section
                                     form:Answer ) ; ] ;
    rdfs:range       form:Question ;
    rdfs:isDefinedBy form: ;
.

form:text
    a                owl:DatatypeProperty ;
    rdfs:label       "text"@en ;
    dct:description  """
        The text property defines the visible question text that will be asked.
        It can also be used to define the text for a given choice.
        In addition to this the usual rdfs:label and dct:description can also be used.
    """@en ;
    rdfs:domain      [ a           owl:Class ;
                       owl:unionOf ( form:Question
                                     form:Choice ) ; ] ;
    rdfs:range       [ a           owl:Class ;
                       owl:unionOf ( xsd:string
                                     rdf:langString ) ; ] ;
    rdfs:isDefinedBy form: ;
.

form:mandatory
    a                owl:DatatypeProperty ;
    rdfs:label       "mandatory"@en ;
    dct:description  """
        This reference indicates a mandatory question.
        For each question type this might mean something different,
        e.g. a text based input must not be empty and a selection must contain at least one choice.
    """@en ;
    rdfs:domain      form:Question ;
    rdfs:range       xsd:boolean ;
    rdfs:isDefinedBy form: ;
.

form:requires
    a                owl:ObjectProperty ;
    rdfs:label       "requires"@en ;
    dct:description  """
        This reference is used to indicate, whether is makes sense to ask a question or not.
        If this property references another question or choice, the referring question should only be asked,
        if the linked question was answered or the linked choice was selected.
    """@en ;
    rdfs:domain      form:Question ;
    rdfs:range       [ a           owl:Class ;
                       owl:unionOf ( form:Question
                                     form:Choice ) ; ] ;
    rdfs:isDefinedBy form: ;
.

form:QuestionnaireResult
    a                owl:Class ;
    rdfs:label       "Questionnaire Result"@en ;
    dct:description  """
        The questionnaire result is the root object that contains all answers.
        In contrast to the questionnaire it does not contain sections, because those are not relevant for the answers.
    """@en ;
    rdfs:isDefinedBy form: ;
.

form:Answer
    a                owl:Class ;
    rdfs:label       "Question"@en ;
    rdfs:isDefinedBy form: ;
.

form:answer
    a                owl:ObjectProperty ;
    rdfs:label       "answer"@en ;
    dct:description  """
        The answer property is used with the questionnaire result class to list the answers.
    """@en ;
    rdfs:domain      [ a           owl:Class ;
                       owl:unionOf ( form:QuestionnaireResult
                                     form:Answer ) ; ] ;
    rdfs:range       form:Answer ;
    rdfs:isDefinedBy form: ;
.

form:InputQuestion
    a                owl:Class ;
    rdfs:subClassOf  form:Question ;
    rdfs:label       "Input Question"@en ;
    dct:description  """
        A type of question which answers are given in form of a text input.
        The visual representation of this question might vary depending on certain properties.
    """@en ;
    rdfs:isDefinedBy form: ;
.

form:placeholder
    a                owl:DatatypeProperty ;
    rdfs:label       "placeholder"@en ;
    dct:description  """
        The placeholder property defines a visible text that will be displayed in an empty text input.
    """@en ;
    rdfs:domain      form:InputQuestion ;
    rdfs:range       [ a           owl:Class ;
                       owl:unionOf ( xsd:string
                                     rdf:langString ) ; ] ;
    rdfs:isDefinedBy form: ;
.

form:datatype
    a                owl:ObjectProperty ;
    rdfs:label       "datatype"@en ;
    dct:description  """
        This reference defines the datatype for a text based input.
        It can be used to specify the type of input that should be used for this question.
    """@en ;
    rdfs:domain      form:InputQuestion ;
    rdfs:range       rdfs:Datatype ;
    rdfs:isDefinedBy form: ;
.

form:pattern
    a                owl:DatatypeProperty ;
    rdfs:label       "pattern"@en ;
    dct:description  """
        This reference defines a required pattern for string inputs.
        The syntax for patterns are regular expressions as defined by xml schema.
    """@en ;
    rdfs:domain      form:InputQuestion ;
    rdfs:range       xsd:string ;
    rdfs:isDefinedBy form: ;
.

form:minLength
    a                owl:DatatypeProperty ;
    rdfs:label       "min length"@en ;
    dct:description  """
        This reference defines a minimum length for string inputs.
    """@en ;
    rdfs:domain      form:InputQuestion ;
    rdfs:range       xsd:nonNegativeInteger ;
    rdfs:isDefinedBy form: ;
.

form:maxLength
    a                owl:DatatypeProperty ;
    rdfs:label       "max length"@en ;
    dct:description  """
        This reference defines a maximum length for string inputs.
    """@en ;
    rdfs:domain      form:InputQuestion ;
    rdfs:range       xsd:nonNegativeInteger ;
    rdfs:isDefinedBy form: ;
.

form:minExclusive
    a                owl:DatatypeProperty ;
    rdfs:label       "min exclusive"@en ;
    dct:description  """
        This reference defines a minimum exclusive value for number inputs.
    """@en ;
    rdfs:domain      form:InputQuestion ;
    rdfs:range       xsd:decimal ;
    rdfs:isDefinedBy form: ;
.

form:minInclusive
    a                owl:DatatypeProperty ;
    rdfs:label       "min inclusive"@en ;
    dct:description  """
        This reference defines a minimum inclusive value for number inputs.
    """@en ;
    rdfs:domain      form:InputQuestion ;
    rdfs:range       xsd:decimal ;
    rdfs:isDefinedBy form: ;
.

form:maxExclusive
    a                owl:DatatypeProperty ;
    rdfs:label       "max exclusive"@en ;
    dct:description  """
        This reference defines a maximum exclusive value for number inputs.
    """@en ;
    rdfs:domain      form:InputQuestion ;
    rdfs:range       xsd:decimal ;
    rdfs:isDefinedBy form: ;
.

form:maxInclusive
    a                owl:DatatypeProperty ;
    rdfs:label       "max inclusive"@en ;
    dct:description  """
        This reference defines a maximum inclusive value for number inputs.
    """@en ;
    rdfs:domain      form:InputQuestion ;
    rdfs:range       xsd:decimal ;
    rdfs:isDefinedBy form: ;
.

form:value
    a                owl:DatatypeProperty ;
    rdfs:label       "value"@en ;
    dct:description  """
        This reference is used to define the answer for a text based question.
    """@en ;
    rdfs:domain      form:Answer ;
    rdfs:range       xsd:string ;
    rdfs:isDefinedBy form: ;
.

form:SelectQuestion
    a                owl:Class ;
    rdfs:subClassOf  form:Question ;
    rdfs:label       "Select Question"@en ;
    dct:description  """
        A type of question which answers are given in form of a selection of choices.
        The visual representation of this question might vary depending on certain properties.
    """@en ;
    rdfs:isDefinedBy form: ;
.

form:Choice
    a                owl:Class ;
    rdfs:label       "Choice"@en ;
    dct:description  """
        The choice is used for select questions and can be referenced by corresponding answer.
    """@en ;
    rdfs:isDefinedBy form: ;
.

form:choice
    a                owl:ObjectProperty ;
    rdfs:label       "choice"@en ;
    dct:description  """
        This reference links a select question to the corresponding choices.
        The same reference is used to link the answer to the selected choice.
    """@en ;
    rdfs:domain      [ a           owl:Class ;
                       owl:unionOf ( form:SelectQuestion
                                     form:Answer ) ; ] ;
    rdfs:range       form:Choice ;
    rdfs:isDefinedBy form: ;
.

form:exclusive
    a                owl:DatatypeProperty ;
    rdfs:label       "exclusive"@en ;
    dct:description  """
        This reference indicates an exclusive selection.
        The visual representation might contain radio buttons or a dropdown instead of checkboxes.
    """@en ;
    rdfs:domain      form:SelectQuestion ;
    rdfs:range       xsd:boolean ;
    rdfs:isDefinedBy form: ;
.

form:TableQuestion
    a                owl:Class ;
    rdfs:subClassOf  form:Question ;
    rdfs:label       "Table"@en ;
    dct:description  """
        A type of question which answers are given in form of table rows.
        Each column in the table consists of another type of question.
        The visual representation of this question might vary depending on certain properties.
    """@en ;
    rdfs:isDefinedBy form: ;
.

form:column
    a                owl:ObjectProperty ;
    rdfs:label       "column"@en ;
    dct:description  """
        This reference links a table question to the corresponding column questions.
    """@en ;
    rdfs:domain      form:TableQuestion ;
    rdfs:range       form:Question ;
    rdfs:isDefinedBy form: ;
.

form:RowAnswer
    a                owl:Class ;
    rdfs:subClassOf  form:Answer ;
    rdfs:label       "Row Answer"@en ;
    dct:description  """
        A type of answer which is used for table questions.
        Each row answer should contain as many column answers as the table question had columns.
    """@en ;
    rdfs:isDefinedBy form: ;
.

form:ColumnAnswer
    a                owl:Class ;
    rdfs:subClassOf  form:Answer ;
    rdfs:label       "Column Answer"@en ;
    dct:description  """
        A type of answer which is used for table questions.
        Each column answer must have a reference to the corresponding column question.
    """@en ;
    rdfs:isDefinedBy form: ;
.

form:minCount
    a                owl:DatatypeProperty ;
    rdfs:label       "min count"@en ;
    dct:description  """
        This reference defines a minimum number of entries for a list of inputs.
    """@en ;
    rdfs:domain      form:TableQuestion ;
    rdfs:range       xsd:nonNegativeInteger ;
    rdfs:isDefinedBy form: ;
.

form:maxCount
    a                owl:DatatypeProperty ;
    rdfs:label       "max count"@en ;
    dct:description  """
        This reference defines a maximum number of entries for a list of inputs.
    """@en ;
    rdfs:domain      form:TableQuestion ;
    rdfs:range       xsd:nonNegativeInteger ;
    rdfs:isDefinedBy form: ;
.
